ver3_less_complex/Trace.dfy
@@ -13,4 +13,18 @@ module M_Trace {
         && (forall i : nat :: && ValidSystemState(t(i))
                               && SystemNext(t(i), t(i+1)))
     }
+
+    ghost predicate Reachable(ss : SystemState)
+    {
+        || SystemInit(ss)
+        || exists run : seq<SystemState> ::
+                                            && |run| > 1
+                                            && SystemInit(run[0])
+                                            && run[|run|-1] == ss
+                                            && (forall i | 0 <= i < |run|-1
+                                                        :: 
+                                                           && ValidSystemState(run[i])
+                                                           && SystemNext(run[i], run[i+1]))
+        
+    }
 }
