ver3_less_complex/Axioms.dfy
@@ -1,0 +1,14 @@
+include "Type.dfy"
+include "Auxilarily.dfy"
+
+module M_Axiom {
+    import opened M_SpecTypes
+    import opened M_AuxilarilyFunc
+
+    lemma{:axiom} Axiom_Common_Constraints()
+    ensures All_Nodes != {}
+
+    lemma{:axiom} Axiom_Byz_Constraints()
+    ensures |Adversary_Nodes| <= f(|All_Nodes|)
+    ensures Adversary_Nodes * Honest_Nodes == {}
+}
