ver3_less_complex/Type.dfy
@@ -2,57 +2,57 @@
 
 module M_SpecTypes {
 
-    type {:extern "Address"} Address(==,!new)
+  type {:extern "Address"} Address(==,!new)
 
 
-    datatype Block = Block(parent : Block) | EmptyBlock
+  datatype Block = Block(parent : Block) | EmptyBlock
 
-    type Blockchain = seq<Block>
+  type Blockchain = seq<Block>
 
 
-    datatype Cert = Cert(
-        cType : MsgType,
-        viewNum : nat,
-        block : Block,
-        signatures : set<Signature>
-    ) | CertNone
-    
-    datatype Signature = Signature(
-        signer : Address,
-        mType : MsgType,
-        viewNum : nat,
-        block : Block
-    ) | SigNone
+  datatype Cert = Cert(
+                    cType : MsgType,
+                    viewNum : nat,
+                    block : Block,
+                    signatures : set<Signature>
+                  ) | CertNone
 
-    datatype MsgType = MT_NewView | MT_Prepare | MT_PreCommit | MT_Commit | MT_Decide
+  datatype Signature = Signature(
+                         signer : Address,
+                         mType : MsgType,
+                         viewNum : nat,
+                         block : Block
+                       ) | SigNone
 
-    
+  datatype MsgType = MT_NewView | MT_Prepare | MT_PreCommit | MT_Commit | MT_Decide
 
-    datatype Msg = Msg(
-        mType : MsgType,
-        viewNum : nat,
-        block : Block,
-        justify : Cert,
-        partialSig : Signature
-    )
 
-    datatype MsgWithRecipient = MsgWithRecipient(
-        msg : Msg,
-        recipient : Address
-    )
-        
-    const Honest_Nodes : set<Address>
 
-    const Adversary_Nodes : set<Address>
+  datatype Msg = Msg(
+    mType : MsgType,
+    viewNum : nat,
+    block : Block,
+    justify : Cert,
+    partialSig : Signature
+  )
 
-    const All_Nodes : set<Address> := Honest_Nodes + Adversary_Nodes
+  datatype MsgWithRecipient = MsgWithRecipient(
+    msg : Msg,
+    recipient : Address
+  )
 
-    const Genesis_Block : Block
-    
-    datatype Configuration = Configuration(
-        honestNodes : set<Address>,
-        adversaryNodes : set<Address>,
-        nodes : set<Address> := honestNodes + adversaryNodes,   // all the nodes, containing byzantine nodes
-        genesisBlock : Block
-    )
+  const Honest_Nodes : set<Address>
+
+  const Adversary_Nodes : set<Address>
+
+  const All_Nodes : set<Address> := Honest_Nodes + Adversary_Nodes
+
+  const Genesis_Block : Block
+
+  datatype Configuration = Configuration(
+    honestNodes : set<Address>,
+    adversaryNodes : set<Address>,
+    nodes : set<Address> := honestNodes + adversaryNodes,   // all the nodes, containing byzantine nodes
+    genesisBlock : Block
+  )
 }
